fstar/treesync/symbolic/MLS.TreeSync.Symbolic.AuthService.fst
@@ -1,0 +1,36 @@
+module MLS.TreeSync.Symbolic.AuthService
+
+open Comparse
+open DY.Core
+open DY.Lib
+open MLS.TreeSync.NetworkTypes
+open MLS.TreeSync.Invariants.AuthService
+open MLS.Symbolic
+
+#set-options "--fuel 0 --ifuel 0"
+
+[@@ with_bytes dy_bytes]
+type dy_as_token = {
+  who: principal;
+  time: nat;
+}
+
+%splice [ps_dy_as_token] (gen_parser (`dy_as_token))
+%splice [ps_dy_as_token_is_well_formed] (gen_is_well_formed_lemma (`dy_as_token))
+
+/// Instantiation of the abstract "Authentication Service" for DY*.
+/// The token is a a principal and a timestamp,
+/// and the AS attests that the signature verification key belonged to that principal at that time.
+val dy_asp: {|crypto_invariants|} -> trace -> as_parameters dy_bytes
+let dy_asp #ci tr = {
+  token_t = dy_as_token;
+  credential_ok = (fun (vk, cred) token ->
+    token.time <= (DY.Core.Trace.Base.length tr) /\
+    bytes_invariant (prefix tr token.time) vk /\
+    vk `has_signkey_usage tr` mk_mls_sigkey_usage token.who /\
+    get_signkey_label tr vk == principal_label token.who
+  );
+  valid_successor = (fun (vk_old, cred_old) (vk_new, cred_new) ->
+    True
+  );
+}
